reflectionDemoScript.sml
@@ -2,6 +2,86 @@ open HolKernel boolLib bossLib lcsymtacs
 open reflectionLib
 val _ = new_theory"reflectionDemo"
 
-val _ = save_thm("example",prop_to_loeb_hyp``0 = 1``)
+val () = show_assums := true
+
+val p = ``0 = 1``
+val res1 = prop_to_loeb_hyp p
+val p = ``∀y. (λx. F) z``
+val res2 = prop_to_loeb_hyp p
+val p = ``(∀y. (λx. F) z) ⇔ ¬z``
+val res3 = prop_to_loeb_hyp p
+
+open basicReflectionLib miscTheory listSimps stringSimps
+open setSpecTheory holSemanticsTheory reflectionTheory pairSyntax listSyntax stringSyntax
+open holBoolTheory holBoolSyntaxTheory holSyntaxExtraTheory
+
+val base_tyval_tm = ``base_tyval``
+
+val (update_list_tm,mk_update_list,dest_update_list,is_update_list)
+  = syntax_fns "misc" 3 dest_triop mk_triop "UPDATE_LIST"
+
+val is_type_valuation_tm = ``is_type_valuation``
+val is_set_theory_mem = ``is_set_theory ^mem``
+
+val mk_is_in = mk_monop``is_in``
+
+val tyval_asms = filter (can (match_term ``^tyval x = range y``)) o hyp
+
+fun mk_tyval th =
+  let
+    val asms = tyval_asms th
+    fun mk_kv eq =
+      let
+        val (l,r) = dest_eq eq
+      in
+        mk_pair(rand l,r)
+      end
+    val pairs = map mk_kv asms
+    val pairs = mk_list(pairs,mk_prod(string_ty,U))
+    val tyval = list_mk_icomb(update_list_tm,[base_tyval_tm,pairs])
+    val is_ins = map (mk_is_in o rand o rand) asms
+    val goal = (is_set_theory_mem::is_ins,mk_comb(is_type_valuation_tm,tyval))
+    val th = TAC_PROOF(goal,
+      match_mp_tac is_type_valuation_update_list >>
+      conj_tac >- ACCEPT_TAC base_tyval_def >>
+      SIMP_TAC (std_ss ++ LIST_ss) [] >>
+      rpt conj_tac >>
+      match_mp_tac inhabited_range >>
+      first_assum ACCEPT_TAC)
+  in
+    SIMP_RULE std_ss [UPDATE_LIST_THM] th
+  end
+
+val tyval_th = mk_tyval res2
+val r3 = res2 |> INST[tyval|->(rand(concl tyval_th))]
+val simpths = mapfilter (QCHANGED_CONV (SIMP_CONV (std_ss++LIST_ss++STRING_ss) [combinTheory.APPLY_UPDATE_THM])) (hyp r3)
+val phyps = map EQT_ELIM simpths
+val r4 = foldl (uncurry PROVE_HYP) r3 phyps
+val r5 = Q.INST[`ctxt`|->`mk_bool_ctxt init_ctxt`] r4
+val bool_insts =
+  bool_sig_instances
+  |> Q.GEN`sig`
+  |> Q.SPEC`sigof(mk_bool_ctxt init_ctxt)`
+  |> SIMP_RULE std_ss []
+val is_bool_sig_goal:goal = ([],fst(dest_imp(concl bool_insts)))
+val is_bool_sig_th = TAC_PROOF(is_bool_sig_goal,
+  match_mp_tac bool_has_bool_sig >>
+  ACCEPT_TAC (MATCH_MP theory_ok_sig init_theory_ok |> SIMP_RULE std_ss []))
+val is_std_sig_goal:goal = ([],first (can (match_term ``is_std_sig x``)) (hyp r5))
+val is_std_sig_th = TAC_PROOF(is_std_sig_goal,
+  match_mp_tac is_bool_sig_std >>
+  ACCEPT_TAC is_bool_sig_th)
+val r6 = PROVE_HYP is_std_sig_th r5
+val bool_insts = MATCH_MP bool_insts is_bool_sig_th
+val bool_sig = is_bool_sig_def
+  |> Q.SPEC`sigof(mk_bool_ctxt init_ctxt)`
+  |> SIMP_RULE std_ss [is_bool_sig_th,is_std_sig_th]
+val simpths = mapfilter (QCHANGED_CONV (SIMP_CONV (std_ss++LIST_ss++STRING_ss)
+  [combinTheory.APPLY_UPDATE_THM,bool_insts,bool_sig,is_instance_refl])) (hyp r6)
+val r7 = foldl (uncurry (C simplify_assum)) r6 simpths |> PROVE_HYP TRUTH
+val simpths = mapfilter (QCHANGED_CONV (SIMP_CONV (std_ss) [is_valuation_def,tyval_th])) (hyp r7)
+val r8 = foldl (uncurry (C simplify_assum)) r7 simpths
+
+val _ = save_thm("example",r8)
 
 val _ = export_theory()
